# 导数

若 $f(x)$ 有导数，则其导数连续

证：$f(x)$ 有导数即 $\lim_{\Delta x \to 0} (\frac{f(x+\Delta x) - f(x)}{\Delta x})$ 存在. 所以
$$
\begin{aligned}
 & \lim_{\Delta x \to 0} (f(x+\Delta x) - f(x)) \\
=& \lim_{\Delta x \to 0}(\frac{f(x+\Delta x) - f(x)}{\Delta x} \cdot \Delta x) \\
=& \lim_{\Delta x \to 0}(\frac{f(x+\Delta x) - f(x)}{\Delta x}) \cdot \lim_{\Delta x \to 0}{\Delta x} \\
=& 0 ,
\end{aligned}
$$
也就是
$$
\lim_{\Delta x \to 0} f(x+\Delta x) = f(x).
$$
得证.



### 导数运算法则

#### 加减法 $(f(x) \pm g(x))' = f'(x) \pm g'(x)$

证明：
$$
\begin{aligned}

 & (f(x) \pm g(x))' \\
=& \lim_{\Delta x \to 0} \frac{(f(x + \Delta x) \pm g(x + \Delta x)) - (f(x) \pm g(x))}{\Delta x} \\
=& \lim_{\Delta x \to 0} \frac{f(x + \Delta x) - f(x)}{\Delta x} \pm \lim_{\Delta x \to 0} \frac{g(x + \Delta x) - g(x)}{\Delta x} \\
=& f'(x) \pm g'(x)

\end{aligned}
$$


#### 乘法 $(f(x)g(x))' = f'(x)g(x) + f(x)g'(x)$

证明：
$$
\begin{aligned}

 & (f(x)g(x))' \\
=& \lim_{\Delta x \to 0} \frac{f(x + \Delta x)g(x + \Delta x) - f(x)g(x)}{\Delta x} \\
=& \lim_{\Delta x \to 0} \frac{f(x + \Delta x)g(x + \Delta x) + f(x + \Delta x)g(x) - f(x + \Delta x)g(x) - f(x)g(x)}{\Delta x} \\
=& \lim_{\Delta x \to 0} \frac{g(x)(f(x + \Delta x) - f(x)) + f(x + \Delta x)(g(x + \Delta x) - g(x))}{\Delta x} \\
=& \lim_{\Delta x \to 0} g(x) \frac{f(x + \Delta x) - f(x)}{\Delta x} + \lim_{\Delta x \to 0} f(x + \Delta x) \frac{g(x + \Delta x) - g(x)}{\Delta x} \\
=& g(x) \lim_{\Delta x \to 0} \frac{f(x + \Delta x) - f(x)}{\Delta x} + f(x) \lim_{\Delta x \to 0} \frac{g(x + \Delta x) - g(x)}{\Delta x} \\
=& f'(x)g(x) + f(x)g'(x)

\end{aligned}
$$

#### 除法

#### 链式法则

